theories/Zmod/Zmod.v
@@ -3,3 +3,4 @@ From Stdlib Require Export ZArith ZModOffset Lia.
 From Stdlib Require Export Zmod.ZmodDef.
 From Stdlib Require Export Zmod.ZmodBase.
 From Stdlib Require Export Zmod.ZmodInv.
+From Stdlib Require Export Zmod.ZmodNsatz.
